theories/Index/Index.v
@@ -1,50 +1,70 @@
+(** * PnVRocqLib *)
+
+(** ** Constructive Theories *)
+
+Require Import PnV.Prelude.SfLib.
+Require Import PnV.Prelude.Notations.
+Require Import PnV.Prelude.PnVTacs.
+Require Import PnV.Prelude.Prelude.
+Require Import PnV.Prelude.ConstructiveFacts.
+Require Import PnV.Prelude.X.
 
 Require Import PnV.Control.Category.
 Require Import PnV.Control.Monad.
 
 Require Import PnV.Data.Aczel.
-Require Import PnV.Data.FiniteMap.
+Require Import PnV.Data.HsOrd.
 Require Import PnV.Data.FiniteSet.
+Require Import PnV.Data.FiniteMap.
 Require Import PnV.Data.Graph.
 Require Import PnV.Data.ITree.
+Require Import PnV.Data.NumRepr.
 Require Import PnV.Data.Vector.
 
 Require Import PnV.Logic.BasicFol.
 Require Import PnV.Logic.BasicFol2.
-Require Import PnV.Logic.ClassicalFol.
-Require Import PnV.Logic.ClassicalPropositionalLogic.
-Require Import PnV.Logic.ExtraFol.
-Require Import PnV.Logic.HELFER1.
-Require Import PnV.Logic.HELFER2.
 Require Import PnV.Logic.HilbertFol.
+Require Import PnV.Logic.ExtraFol.
 Require Import PnV.Logic.HilbertFol2.
-Require Import PnV.Logic.MuRec.
+Require Import PnV.Logic.HELFER1.
 Require Import PnV.Logic.PrimRec.
+Require Import PnV.Logic.MuRec.
 Require Import PnV.Logic.PropositionalLogic.
 
 Require Import PnV.Math.BasicTopology.
-Require Import PnV.Math.BooleanAlgebra.
-Require Import PnV.Math.ClassicalDomainTheory.
-Require Import PnV.Math.ClassicalSetTheory.
-Require Import PnV.Math.DomainTheory.
 Require Import PnV.Math.OrderTheory.
+Require Import PnV.Math.BooleanAlgebra.
+Require Import PnV.Math.DomainTheory.
 Require Import PnV.Math.SetTheory.
 Require Import PnV.Math.ThN.
 
-Require Import PnV.Prelude.ClassicalFacts.
-Require Import PnV.Prelude.ConstructiveFacts.
-Require Import PnV.Prelude.Notations.
-Require Import PnV.Prelude.Prelude.
-Require Import PnV.Prelude.Quotient.
-Require Import PnV.Prelude.SfLib.
-Require Import PnV.Prelude.X.
-
 Require Import PnV.System.BasicITreeTh.
-Require Import PnV.System.FolFramework.
+Require Import PnV.System.LGS.
+Require Import PnV.System.LGSSem.
+Require Import PnV.System.LGSCorrect.
+Require Import PnV.System.P.
 Require Import PnV.System.Lambda1.
 Require Import PnV.System.Lang.
-Require Import PnV.System.LGS.
-Require Import PnV.System.P.
 Require Import PnV.System.PGS.
+Require Import PnV.System.PGSSem.
+Require Import PnV.System.PGSCorrect.
 Require Import PnV.System.Regex.
 Require Import PnV.System.STLC.
+
+(** ** Classical Theories *)
+
+Require Import PnV.Prelude.ClassicalFacts.
+
+Require Import PnV.Logic.ClassicalFol.
+Require Import PnV.Logic.ClassicalPropositionalLogic.
+Require Import PnV.Logic.HELFER2.
+
+Require Import PnV.Math.ClassicalSetTheory.
+Require Import PnV.Math.ClassicalCardinal.
+Require Import PnV.Math.ClassicalDomainTheory.
+
+Require Import PnV.System.FolFramework.
+
+(** ** Theories with Quotient Types *)
+
+Require Import PnV.Prelude.Quotient.
