theories/Prelude/PnVTacs.v
@@ -1,0 +1,415 @@
+Require Export Stdlib.micromega.Lia.
+Require Import PnV.Prelude.Notations.
+Require Export PnV.Prelude.SfLib.
+
+Tactic Notation "rewrite*" uconstr( t ) "by" ident ( H_EQ ) :=
+  let lhs := fresh "lhs" in
+  set (lhs := t) in |- *;
+  match type of H_EQ with
+  | ?X = ?Y => change (lhs = Y) in H_EQ; rewrite -> H_EQ; subst lhs
+  end.
+
+Tactic Notation "find" simple_intropattern( p ) "by" uconstr( H ) :=
+  unshelve hexploit H; [eauto .. | intros p].
+
+Tactic Notation "find*" simple_intropattern( p ) "by" uconstr( H ) :=
+  hexploit H; [eauto .. | intros p].
+
+Module Tac_obtaion_private.
+
+Definition _Tag (cnt : nat) : Set :=
+  unit.
+
+#[universes(template), projections(primitive)]
+Record _TaggedLock (tag : nat) (A : Type) : Type :=
+  _mkTaggedLock { _unTaggedLock : A } as lock.
+
+#[global] Arguments _mkTaggedLock {tag} {A}.
+#[global] Arguments _unTaggedLock {tag} {A} lock.
+
+Ltac new_tag_cnt :=
+  let TAG_cnt := fresh "TAG_cnt" in
+  refine (let TAG_cnt : _Tag 0 := tt in _);
+  clearbody TAG_cnt.
+
+Ltac load arg :=
+  let Shelf := fresh "Shelf" in
+  match goal with
+  | [ TAG_cnt : _Tag ?n |- _ ] =>
+    refine (let Shelf : _TaggedLock n _ := _mkTaggedLock arg in _);
+    change (_Tag (S n)) in TAG_cnt
+  end.
+
+Ltac free_all :=
+  repeat (
+    match goal with
+    | [ Shelf : _TaggedLock _ _ |- _ ] => subst Shelf
+    end
+  );
+  repeat (
+    match goal with
+    | [ TAG_cnt : _Tag _ |- _ ] => clear TAG_cnt
+    end
+  ).
+
+Ltac isSort A :=
+  lazymatch A with
+  | Set => idtac
+  | Type => idtac
+  | Prop => idtac
+  | SProp => idtac
+  | _ => fail
+  end.
+
+Ltac unify_arg_type expected actual :=
+  first
+  [ unify expected actual
+  | isSort expected;
+    isSort actual
+  ].
+
+Ltac xapply idx prf :=
+  lazymatch type of prf with
+  | forall x : ?A, _ =>
+    first
+    [ lazymatch goal with
+      | [ Shelf := @_mkTaggedLock _ ?A' ?arg : _TaggedLock idx _ |- _ ] =>
+        unify_arg_type A A';
+        xapply constr:(S idx) (prf arg)
+      end
+    | isSort A;
+      let _RET_ := fresh "_RET_" in
+      epose proof (prf _) as _RET_;
+      xapply idx _RET_;
+      clear _RET_
+    | let _RET_ := fresh "_RET_" in
+      unshelve epose proof (prf _) as _RET_;
+      [ idtac
+      | xapply idx _RET_;
+        clear _RET_
+      ]
+    ]
+  | let _ := _ in _ =>
+    let _RET_ := fresh "_RET_" in
+    epose proof prf as _RET_;
+    cbv zeta in _RET_;
+    xapply idx _RET_;
+    clear _RET_
+  | _ =>
+    match goal with
+    | [ TAG_cnt : _Tag ?total |- _ ] =>
+      first
+      [ constr_eq idx total
+      | fail 1 "obtain: not all supplied arguments were consumed"
+      ]
+    end;
+    let _RET_ := fresh "_RET_" in
+    epose proof (_RET_ := prf);
+    revert _RET_
+  end.
+
+Ltac fire func :=
+  let _RET_ := fresh "_RET_" in
+  epose proof func as _RET_;
+  xapply constr:(0) _RET_;
+  try clear _RET_;
+  free_all.
+
+Ltac last :=
+  first
+  [ typeclasses eauto
+  | congruence
+  | tauto
+  | lia
+  | eauto
+  ].
+
+End Tac_obtaion_private.
+
+Tactic Notation "obtain" simple_intropattern( ret ) "with" "*" "by" uconstr( func ) :=
+  find* ret by func.
+
+Tactic Notation "obtain" simple_intropattern( ret ) "with" uconstr( arg1 ) "by" uconstr( func ) :=
+  Tac_obtaion_private.new_tag_cnt;
+  Tac_obtaion_private.load arg1;
+  Tac_obtaion_private.fire func;
+  [Tac_obtaion_private.last.. | intros ret].
+
+Tactic Notation "obtain" simple_intropattern( ret ) "with" uconstr( arg1 ) uconstr( arg2 ) "by" uconstr( func ) :=
+  Tac_obtaion_private.new_tag_cnt;
+  Tac_obtaion_private.load arg1;
+  Tac_obtaion_private.load arg2;
+  Tac_obtaion_private.fire func;
+  [Tac_obtaion_private.last.. | intros ret].
+
+Tactic Notation "obtain" simple_intropattern( ret ) "with" uconstr( arg1 ) uconstr( arg2 ) uconstr( arg3 ) "by" uconstr( func ) :=
+  Tac_obtaion_private.new_tag_cnt;
+  Tac_obtaion_private.load arg1;
+  Tac_obtaion_private.load arg2;
+  Tac_obtaion_private.load arg3;
+  Tac_obtaion_private.fire func;
+  [Tac_obtaion_private.last.. | intros ret].
+
+Tactic Notation "obtain" simple_intropattern( ret ) "with" uconstr( arg1 ) uconstr( arg2 ) uconstr( arg3 ) uconstr( arg4 ) "by" uconstr( func ) :=
+  Tac_obtaion_private.new_tag_cnt;
+  Tac_obtaion_private.load arg1;
+  Tac_obtaion_private.load arg2;
+  Tac_obtaion_private.load arg3;
+  Tac_obtaion_private.load arg4;
+  Tac_obtaion_private.fire func;
+  [Tac_obtaion_private.last.. | intros ret].
+
+Tactic Notation "obtain" simple_intropattern( ret ) "with" uconstr( arg1 ) uconstr( arg2 ) uconstr( arg3 ) uconstr( arg4 ) uconstr( arg5 ) "by" uconstr( func ) :=
+  Tac_obtaion_private.new_tag_cnt;
+  Tac_obtaion_private.load arg1;
+  Tac_obtaion_private.load arg2;
+  Tac_obtaion_private.load arg3;
+  Tac_obtaion_private.load arg4;
+  Tac_obtaion_private.load arg5;
+  Tac_obtaion_private.fire func;
+  [Tac_obtaion_private.last.. | intros ret].
+
+Tactic Notation "obtain" simple_intropattern( ret ) "with" uconstr( arg1 ) uconstr( arg2 ) uconstr( arg3 ) uconstr( arg4 ) uconstr( arg5 ) uconstr( arg6 ) "by" uconstr( func ) :=
+  Tac_obtaion_private.new_tag_cnt;
+  Tac_obtaion_private.load arg1;
+  Tac_obtaion_private.load arg2;
+  Tac_obtaion_private.load arg3;
+  Tac_obtaion_private.load arg4;
+  Tac_obtaion_private.load arg5;
+  Tac_obtaion_private.load arg6;
+  Tac_obtaion_private.fire func;
+  [Tac_obtaion_private.last.. | intros ret].
+
+Tactic Notation "obtain" simple_intropattern( ret ) "with" uconstr( arg1 ) uconstr( arg2 ) uconstr( arg3 ) uconstr( arg4 ) uconstr( arg5 ) uconstr( arg6 ) uconstr( arg7 ) "by" uconstr( func ) :=
+  Tac_obtaion_private.new_tag_cnt;
+  Tac_obtaion_private.load arg1;
+  Tac_obtaion_private.load arg2;
+  Tac_obtaion_private.load arg3;
+  Tac_obtaion_private.load arg4;
+  Tac_obtaion_private.load arg5;
+  Tac_obtaion_private.load arg6;
+  Tac_obtaion_private.load arg7;
+  Tac_obtaion_private.fire func;
+  [Tac_obtaion_private.last.. | intros ret].
+
+Tactic Notation "obtain" simple_intropattern( ret ) "with" uconstr( arg1 ) uconstr( arg2 ) uconstr( arg3 ) uconstr( arg4 ) uconstr( arg5 ) uconstr( arg6 ) uconstr( arg7 ) uconstr( arg8 ) "by" uconstr( func ) :=
+  Tac_obtaion_private.new_tag_cnt;
+  Tac_obtaion_private.load arg1;
+  Tac_obtaion_private.load arg2;
+  Tac_obtaion_private.load arg3;
+  Tac_obtaion_private.load arg4;
+  Tac_obtaion_private.load arg5;
+  Tac_obtaion_private.load arg6;
+  Tac_obtaion_private.load arg7;
+  Tac_obtaion_private.load arg8;
+  Tac_obtaion_private.fire func;
+  [Tac_obtaion_private.last.. | intros ret].
+
+Tactic Notation "obtain" simple_intropattern( ret ) "with" uconstr( arg1 ) uconstr( arg2 ) uconstr( arg3 ) uconstr( arg4 ) uconstr( arg5 ) uconstr( arg6 ) uconstr( arg7 ) uconstr( arg8 ) uconstr( arg9 ) "by" uconstr( func ) :=
+  Tac_obtaion_private.new_tag_cnt;
+  Tac_obtaion_private.load arg1;
+  Tac_obtaion_private.load arg2;
+  Tac_obtaion_private.load arg3;
+  Tac_obtaion_private.load arg4;
+  Tac_obtaion_private.load arg5;
+  Tac_obtaion_private.load arg6;
+  Tac_obtaion_private.load arg7;
+  Tac_obtaion_private.load arg8;
+  Tac_obtaion_private.load arg9;
+  Tac_obtaion_private.fire func;
+  [Tac_obtaion_private.last.. | intros ret].
+
+Tactic Notation "obtain" simple_intropattern( ret ) "with" uconstr( arg1 ) uconstr( arg2 ) uconstr( arg3 ) uconstr( arg4 ) uconstr( arg5 ) uconstr( arg6 ) uconstr( arg7 ) uconstr( arg8 ) uconstr( arg9 ) uconstr( arg10 ) "by" uconstr( func ) :=
+  Tac_obtaion_private.new_tag_cnt;
+  Tac_obtaion_private.load arg1;
+  Tac_obtaion_private.load arg2;
+  Tac_obtaion_private.load arg3;
+  Tac_obtaion_private.load arg4;
+  Tac_obtaion_private.load arg5;
+  Tac_obtaion_private.load arg6;
+  Tac_obtaion_private.load arg7;
+  Tac_obtaion_private.load arg8;
+  Tac_obtaion_private.load arg9;
+  Tac_obtaion_private.load arg10;
+  Tac_obtaion_private.fire func;
+  [Tac_obtaion_private.last.. | intros ret].
+
+Tactic Notation "obtain" simple_intropattern( ret ) "with" uconstr( arg1 ) uconstr( arg2 ) uconstr( arg3 ) uconstr( arg4 ) uconstr( arg5 ) uconstr( arg6 ) uconstr( arg7 ) uconstr( arg8 ) uconstr( arg9 ) uconstr( arg10 ) uconstr( arg11 ) "by" uconstr( func ) :=
+  Tac_obtaion_private.new_tag_cnt;
+  Tac_obtaion_private.load arg1;
+  Tac_obtaion_private.load arg2;
+  Tac_obtaion_private.load arg3;
+  Tac_obtaion_private.load arg4;
+  Tac_obtaion_private.load arg5;
+  Tac_obtaion_private.load arg6;
+  Tac_obtaion_private.load arg7;
+  Tac_obtaion_private.load arg8;
+  Tac_obtaion_private.load arg9;
+  Tac_obtaion_private.load arg10;
+  Tac_obtaion_private.load arg11;
+  Tac_obtaion_private.fire func;
+  [Tac_obtaion_private.last.. | intros ret].
+
+Tactic Notation "obtain" simple_intropattern( ret ) "with" uconstr( arg1 ) uconstr( arg2 ) uconstr( arg3 ) uconstr( arg4 ) uconstr( arg5 ) uconstr( arg6 ) uconstr( arg7 ) uconstr( arg8 ) uconstr( arg9 ) uconstr( arg10 ) uconstr( arg11 ) uconstr( arg12 ) "by" uconstr( func ) :=
+  Tac_obtaion_private.new_tag_cnt;
+  Tac_obtaion_private.load arg1;
+  Tac_obtaion_private.load arg2;
+  Tac_obtaion_private.load arg3;
+  Tac_obtaion_private.load arg4;
+  Tac_obtaion_private.load arg5;
+  Tac_obtaion_private.load arg6;
+  Tac_obtaion_private.load arg7;
+  Tac_obtaion_private.load arg8;
+  Tac_obtaion_private.load arg9;
+  Tac_obtaion_private.load arg10;
+  Tac_obtaion_private.load arg11;
+  Tac_obtaion_private.load arg12;
+  Tac_obtaion_private.fire func;
+  [Tac_obtaion_private.last.. | intros ret].
+
+Tactic Notation "obtain" simple_intropattern( ret ) "with" uconstr( arg1 ) uconstr( arg2 ) uconstr( arg3 ) uconstr( arg4 ) uconstr( arg5 ) uconstr( arg6 ) uconstr( arg7 ) uconstr( arg8 ) uconstr( arg9 ) uconstr( arg10 ) uconstr( arg11 ) uconstr( arg12 ) uconstr( arg13 ) "by" uconstr( func ) :=
+  Tac_obtaion_private.new_tag_cnt;
+  Tac_obtaion_private.load arg1;
+  Tac_obtaion_private.load arg2;
+  Tac_obtaion_private.load arg3;
+  Tac_obtaion_private.load arg4;
+  Tac_obtaion_private.load arg5;
+  Tac_obtaion_private.load arg6;
+  Tac_obtaion_private.load arg7;
+  Tac_obtaion_private.load arg8;
+  Tac_obtaion_private.load arg9;
+  Tac_obtaion_private.load arg10;
+  Tac_obtaion_private.load arg11;
+  Tac_obtaion_private.load arg12;
+  Tac_obtaion_private.load arg13;
+  Tac_obtaion_private.fire func;
+  [Tac_obtaion_private.last.. | intros ret].
+
+Tactic Notation "obtain" simple_intropattern( ret ) "with" uconstr( arg1 ) uconstr( arg2 ) uconstr( arg3 ) uconstr( arg4 ) uconstr( arg5 ) uconstr( arg6 ) uconstr( arg7 ) uconstr( arg8 ) uconstr( arg9 ) uconstr( arg10 ) uconstr( arg11 ) uconstr( arg12 ) uconstr( arg13 ) uconstr( arg14 ) "by" uconstr( func ) :=
+  Tac_obtaion_private.new_tag_cnt;
+  Tac_obtaion_private.load arg1;
+  Tac_obtaion_private.load arg2;
+  Tac_obtaion_private.load arg3;
+  Tac_obtaion_private.load arg4;
+  Tac_obtaion_private.load arg5;
+  Tac_obtaion_private.load arg6;
+  Tac_obtaion_private.load arg7;
+  Tac_obtaion_private.load arg8;
+  Tac_obtaion_private.load arg9;
+  Tac_obtaion_private.load arg10;
+  Tac_obtaion_private.load arg11;
+  Tac_obtaion_private.load arg12;
+  Tac_obtaion_private.load arg13;
+  Tac_obtaion_private.load arg14;
+  Tac_obtaion_private.fire func;
+  [Tac_obtaion_private.last.. | intros ret].
+
+Tactic Notation "obtain" simple_intropattern( ret ) "with" uconstr( arg1 ) uconstr( arg2 ) uconstr( arg3 ) uconstr( arg4 ) uconstr( arg5 ) uconstr( arg6 ) uconstr( arg7 ) uconstr( arg8 ) uconstr( arg9 ) uconstr( arg10 ) uconstr( arg11 ) uconstr( arg12 ) uconstr( arg13 ) uconstr( arg14 ) uconstr( arg15 ) "by" uconstr( func ) :=
+  Tac_obtaion_private.new_tag_cnt;
+  Tac_obtaion_private.load arg1;
+  Tac_obtaion_private.load arg2;
+  Tac_obtaion_private.load arg3;
+  Tac_obtaion_private.load arg4;
+  Tac_obtaion_private.load arg5;
+  Tac_obtaion_private.load arg6;
+  Tac_obtaion_private.load arg7;
+  Tac_obtaion_private.load arg8;
+  Tac_obtaion_private.load arg9;
+  Tac_obtaion_private.load arg10;
+  Tac_obtaion_private.load arg11;
+  Tac_obtaion_private.load arg12;
+  Tac_obtaion_private.load arg13;
+  Tac_obtaion_private.load arg14;
+  Tac_obtaion_private.load arg15;
+  Tac_obtaion_private.fire func;
+  [Tac_obtaion_private.last.. | intros ret].
+
+Tactic Notation "obtain" simple_intropattern( ret ) "with" uconstr( arg1 ) uconstr( arg2 ) uconstr( arg3 ) uconstr( arg4 ) uconstr( arg5 ) uconstr( arg6 ) uconstr( arg7 ) uconstr( arg8 ) uconstr( arg9 ) uconstr( arg10 ) uconstr( arg11 ) uconstr( arg12 ) uconstr( arg13 ) uconstr( arg14 ) uconstr( arg15 ) uconstr( arg16 ) "by" uconstr( func ) :=
+  Tac_obtaion_private.new_tag_cnt;
+  Tac_obtaion_private.load arg1;
+  Tac_obtaion_private.load arg2;
+  Tac_obtaion_private.load arg3;
+  Tac_obtaion_private.load arg4;
+  Tac_obtaion_private.load arg5;
+  Tac_obtaion_private.load arg6;
+  Tac_obtaion_private.load arg7;
+  Tac_obtaion_private.load arg8;
+  Tac_obtaion_private.load arg9;
+  Tac_obtaion_private.load arg10;
+  Tac_obtaion_private.load arg11;
+  Tac_obtaion_private.load arg12;
+  Tac_obtaion_private.load arg13;
+  Tac_obtaion_private.load arg14;
+  Tac_obtaion_private.load arg15;
+  Tac_obtaion_private.load arg16;
+  Tac_obtaion_private.fire func;
+  [Tac_obtaion_private.last.. | intros ret].
+
+Tactic Notation "obtain" simple_intropattern( ret ) "with" uconstr( arg1 ) uconstr( arg2 ) uconstr( arg3 ) uconstr( arg4 ) uconstr( arg5 ) uconstr( arg6 ) uconstr( arg7 ) uconstr( arg8 ) uconstr( arg9 ) uconstr( arg10 ) uconstr( arg11 ) uconstr( arg12 ) uconstr( arg13 ) uconstr( arg14 ) uconstr( arg15 ) uconstr( arg16 ) uconstr( arg17 ) "by" uconstr( func ) :=
+  Tac_obtaion_private.new_tag_cnt;
+  Tac_obtaion_private.load arg1;
+  Tac_obtaion_private.load arg2;
+  Tac_obtaion_private.load arg3;
+  Tac_obtaion_private.load arg4;
+  Tac_obtaion_private.load arg5;
+  Tac_obtaion_private.load arg6;
+  Tac_obtaion_private.load arg7;
+  Tac_obtaion_private.load arg8;
+  Tac_obtaion_private.load arg9;
+  Tac_obtaion_private.load arg10;
+  Tac_obtaion_private.load arg11;
+  Tac_obtaion_private.load arg12;
+  Tac_obtaion_private.load arg13;
+  Tac_obtaion_private.load arg14;
+  Tac_obtaion_private.load arg15;
+  Tac_obtaion_private.load arg16;
+  Tac_obtaion_private.load arg17;
+  Tac_obtaion_private.fire func;
+  [Tac_obtaion_private.last.. | intros ret].
+
+Tactic Notation "obtain" simple_intropattern( ret ) "with" uconstr( arg1 ) uconstr( arg2 ) uconstr( arg3 ) uconstr( arg4 ) uconstr( arg5 ) uconstr( arg6 ) uconstr( arg7 ) uconstr( arg8 ) uconstr( arg9 ) uconstr( arg10 ) uconstr( arg11 ) uconstr( arg12 ) uconstr( arg13 ) uconstr( arg14 ) uconstr( arg15 ) uconstr( arg16 ) uconstr( arg17 ) uconstr( arg18 ) "by" uconstr( func ) :=
+  Tac_obtaion_private.new_tag_cnt;
+  Tac_obtaion_private.load arg1;
+  Tac_obtaion_private.load arg2;
+  Tac_obtaion_private.load arg3;
+  Tac_obtaion_private.load arg4;
+  Tac_obtaion_private.load arg5;
+  Tac_obtaion_private.load arg6;
+  Tac_obtaion_private.load arg7;
+  Tac_obtaion_private.load arg8;
+  Tac_obtaion_private.load arg9;
+  Tac_obtaion_private.load arg10;
+  Tac_obtaion_private.load arg11;
+  Tac_obtaion_private.load arg12;
+  Tac_obtaion_private.load arg13;
+  Tac_obtaion_private.load arg14;
+  Tac_obtaion_private.load arg15;
+  Tac_obtaion_private.load arg16;
+  Tac_obtaion_private.load arg17;
+  Tac_obtaion_private.load arg18;
+  Tac_obtaion_private.fire func;
+  [Tac_obtaion_private.last.. | intros ret].
+
+Tactic Notation "obtain" simple_intropattern( ret ) "with" uconstr( arg1 ) uconstr( arg2 ) uconstr( arg3 ) uconstr( arg4 ) uconstr( arg5 ) uconstr( arg6 ) uconstr( arg7 ) uconstr( arg8 ) uconstr( arg9 ) uconstr( arg10 ) uconstr( arg11 ) uconstr( arg12 ) uconstr( arg13 ) uconstr( arg14 ) uconstr( arg15 ) uconstr( arg16 ) uconstr( arg17 ) uconstr( arg18 ) uconstr( arg19 ) "by" uconstr( func ) :=
+  Tac_obtaion_private.new_tag_cnt;
+  Tac_obtaion_private.load arg1;
+  Tac_obtaion_private.load arg2;
+  Tac_obtaion_private.load arg3;
+  Tac_obtaion_private.load arg4;
+  Tac_obtaion_private.load arg5;
+  Tac_obtaion_private.load arg6;
+  Tac_obtaion_private.load arg7;
+  Tac_obtaion_private.load arg8;
+  Tac_obtaion_private.load arg9;
+  Tac_obtaion_private.load arg10;
+  Tac_obtaion_private.load arg11;
+  Tac_obtaion_private.load arg12;
+  Tac_obtaion_private.load arg13;
+  Tac_obtaion_private.load arg14;
+  Tac_obtaion_private.load arg15;
+  Tac_obtaion_private.load arg16;
+  Tac_obtaion_private.load arg17;
+  Tac_obtaion_private.load arg18;
+  Tac_obtaion_private.load arg19;
+  Tac_obtaion_private.fire func;
+  [Tac_obtaion_private.last.. | intros ret].
